WIP list validity

theories/Substitution/Introductions/List.v
@@ -125,586 +125,277 @@ Proof.
       now eapply UnivEq'.
 Qed.
 
-
-Lemma natTermValid {Γ} (VΓ : [||-v Γ]):  [Γ ||-v<one> tNat : U | VΓ | UValid VΓ].
+Lemma nilRed {Γ A l}
+  (RA: [Γ ||-< l > A])
+  (RLA: [Γ ||-< l > tList A]) :
+  [RLA | Γ ||- tNil A : tList A].
 Proof.
-  constructor; intros.
-  - eapply natTermRed. 
-  - eexists (natTermRed wfΔ) (natTermRed wfΔ) (natRed wfΔ); cbn.
-    + gen_typing.
-    + now eapply (natRed (l:=zero)).
-    + constructor; eapply redtywf_refl; gen_typing.
-Qed.
-
-Lemma zeroRed {Γ l} {NN : [Γ ||-Nat tNat]} (wfΓ : [|- Γ]): [Γ ||-<l> tZero : _ | LRNat_ l NN].
-Proof.
-  exists tZero.
-  1,2: gen_typing.
-  constructor.
-Defined.
-
-Lemma zeroRedEq {Γ l} {NN : [Γ ||-Nat tNat]} (wfΓ : [|- Γ]): [Γ ||-<l> tZero ≅ tZero : _ | LRNat_ l NN].
-Proof.
-  exists tZero tZero.
-  1-3: gen_typing.
-  constructor.
-Defined.
-
-Lemma zeroValid {Γ l} (VΓ : [||-v Γ]): 
-  [Γ ||-v<l> tZero : tNat | VΓ | natValid VΓ].
-Proof.
-  constructor; intros; cbn; [unshelve eapply zeroRed| unshelve eapply zeroRedEq]; tea.
-Qed.
-
-Lemma succRed {Γ l n} {NN : [Γ ||-Nat tNat]} :
-  [Γ ||-<l> n : _ | LRNat_ l NN] ->
-  [Γ ||-<l> tSucc n : _ | LRNat_ l NN].
-Proof.
-  intros Rn; exists (tSucc n).
-  + eapply redtmwf_refl; eapply ty_succ; now escape.
-  + eapply convtm_succ; eapply escapeEqTerm; now eapply LREqTermRefl_.
-  + now constructor.
-Defined.
-
-Lemma succRedEq {Γ l n n'} {NN : [Γ ||-Nat tNat]} :
-  [Γ ||-<l> n : _ | LRNat_ l NN] ->
-  [Γ ||-<l> n' : _ | LRNat_ l NN] ->
-  [Γ ||-<l> n ≅ n' : _ | LRNat_ l NN] ->
-  [Γ ||-<l> tSucc n ≅ tSucc n' : _ | LRNat_ l NN].
-Proof.
-  intros ???; escape; exists (tSucc n) (tSucc n').
-  1,2: eapply redtmwf_refl; now eapply ty_succ.
-  + now eapply convtm_succ.
-  + now constructor.
-Defined.
-
-Lemma succRedInv {Γ l n} {NN : [Γ ||-Nat tNat]} :
-  [Γ ||-<l> tSucc n : _ | LRNat_ l NN] ->
-  [Γ ||-<l> n : _ | LRNat_ l NN].
-Proof.
-  intros RSn; inversion RSn; subst. 
-  unshelve epose proof (redtmwf_whnf red _). 1: constructor.
-  subst. inversion prop; subst; tea.
-  match goal with H : [ _ ||-NeNf _ : _] |- _ => destruct H; apply tm_ne_whne in ne; inv_whne end.
-Qed.
-
-Lemma succValid {Γ l n} (VΓ : [||-v Γ]) 
-  (Vn : [Γ ||-v<l> n : tNat | VΓ | natValid VΓ]) :
-  [Γ ||-v<l> tSucc n : tNat | VΓ | natValid VΓ].
-Proof.
-  constructor; intros; cbn.
-  - instValid Vσ ; now unshelve eapply succRed.
-  - instAllValid Vσ Vσ' Vσσ'; now unshelve eapply succRedEq.
-Qed.
-
-Lemma succcongValid {Γ l n n'} (VΓ : [||-v Γ]) 
-  (Vn : [Γ ||-v<l> n : tNat | VΓ | natValid VΓ])
-  (Vn' : [Γ ||-v<l> n' : tNat | VΓ | natValid VΓ])
-  (Veqn : [Γ ||-v<l> n ≅ n' : tNat | VΓ | natValid VΓ]) :
-  [Γ ||-v<l> tSucc n ≅ tSucc n' : tNat | VΓ | natValid VΓ].
-Proof.
-  constructor; intros; cbn; instValid Vσ; now unshelve eapply succRedEq.
-Qed.
-
-Lemma red_natElimSubst {Γ l P hz hs n n'} :
-  [|- Γ] ->
-  [Γ ,, tNat |- P] ->
-  [Γ |- hz : P[tZero..]] ->
-  [Γ |- hs : elimSuccHypTy P] ->
-  [Γ |- n :⇒*: n' : tNat ] ->
-  forall (RN : [Γ ||-<l> tNat]),
-  [Γ ||-<l> n' : tNat | RN] ->
-  (forall t t',
-    [Γ ||-<l> t : tNat | RN] ->
-    [Γ ||-<l> t' : tNat | RN] ->
-    [Γ ||-<l> t ≅ t' : tNat | RN] ->
-    [Γ |- P[t..] ≅ P[t'..]]) -> 
-  [Γ |- tNatElim P hz hs n :⇒*: tNatElim P hz hs n' : P[n..]].
-Proof.
-  intros hΓ hp hhz hhs red rN rn' congP.
-  generalize (tmr_wf_red _ _ _ _ red).
-  escape.
-  assert ([rN | Γ ||- n : tNat]).
-  { now eapply redwfSubstTerm. }
-  assert ([ Γ |- P[n..] ≅ P[n'..]]).
-  { apply congP; [assumption|assumption|].
-    now eapply redwfSubstTerm. }
-  intros.
+  enough [ normList RLA | Γ ||- tNil A : _] by irrelevance.
   econstructor.
-  - eapply ty_conv; [|now symmetry].
-    escape; apply ty_natElim; tea.
-  - apply redtm_natelim; tea.
-    + now eapply redtm_ty_src.
-    + intros u Hu.
-      assert ([Γ |-[ ta ] u :⇒*: n' : tNat]).
-      { now constructor. }
-      apply congP; [eassumption| |].
-      * eapply redwfSubstTerm; [exact rn'|assumption].
-      * now eapply LRTmEqSym, redwfSubstTerm.
+  + eapply redtmwf_refl. escape. now apply ty_nil.
+  + eapply convtm_nil. unshelve eapply escapeEq ; tea.
+    apply LRTyEqRefl_.
+  + constructor. 1: escape ; tea.
+    apply LRTyEqRefl_.
 Qed.
 
-Lemma arr_subst_eq {A B σ} : (arr A B)[σ] = arr A[σ] B[σ].
-Proof. now bsimpl. Qed.
-
-Lemma shift_up_eq {t σ} : t⟨↑⟩[up_term_term σ] = t[σ]⟨↑⟩.
-Proof. now bsimpl. Qed.
-
-Lemma up_single_subst {t σ u} : t[up_term_term σ][u..] = t[u .:  σ].
-Proof.  now bsimpl. Qed.
-
-Lemma up_liftSubst_eq {σ t u} : t[up_term_term σ][u]⇑ = t[u .: ↑ >> up_term_term σ].
+Lemma nilEqRed {Γ A A' l}
+  (RA: [Γ ||-< l > A])
+  (RA': [Γ ||-< l > A'])
+  (RLA: [Γ ||-< l > tList A])
+  (RLA': [Γ ||-< l > tList A']) :
+  [RA | Γ ||- A ≅ A'] ->
+  [RLA | Γ ||- tList A ≅ tList A'] ->
+  [RLA | Γ ||- tNil A ≅ tNil A' : tList A].
 Proof.
-  bsimpl. eapply ext_term; intros [|n]; cbn.
-  1: reflexivity.
-  unfold funcomp; now rewrite  rinstInst'_term.
+  intros.
+  enough [normList RLA | Γ ||- tNil A ≅ tNil A' : tList A] by irrelevance.
+  econstructor.
+  (* + eapply redtmwf_refl. escape. now apply ty_nil. *)
+  (* + eapply redtmwf_refl. escape. *)
+  (*   eapply ty_conv. 2: symmetry ; eassumption. *)
+  (*   now eapply ty_nil. *)
+  (* + eapply convtm_nil. escape. eassumption. *)
+  (* + constructor ; escape ; tea. *)
+  (*   - apply LRTyEqRefl_. *)
+  (*   - irrelevance. *)
+Admitted.
+
+Lemma nilValid {Γ A l}
+  {VΓ : [||-v Γ]}
+  {VA : [Γ ||-v<l> A | VΓ]}
+  {VLA : [Γ ||-v<l> tList A | VΓ]} :
+  [Γ ||-v<l> tNil A : tList A | VΓ | VLA].
+Proof.
+  split; intros.
+  - instValid Vσ.
+    now eapply nilRed.
+  - instAllValid Vσ Vσ' Vσσ'.
+    now eapply nilEqRed.
 Qed.
 
-Lemma elimSuccHypTy_subst {P} σ :
-  elimSuccHypTy P[up_term_term σ] = (elimSuccHypTy P)[σ].
+Lemma consRed {Γ A hd tl l}
+  (RA: [Γ ||-< l > A])
+  (RLA: [Γ ||-< l > tList A]) :
+  [RA | Γ ||- hd : A] ->
+  [RLA | Γ ||- tl : tList A] ->
+  [RLA | Γ ||- tCons A hd tl : tList A ].
 Proof.
-  unfold elimSuccHypTy.
-  cbn. rewrite shift_up_eq.
-  rewrite liftSubstComm. cbn. 
-  now rewrite up_liftSubst_eq.
+  intros.
+  enough [ normList RLA | Γ ||- tCons A hd tl : _] by irrelevance.
+  econstructor.
+  + eapply redtmwf_refl. escape. now apply ty_cons.
+  + eapply convtm_cons.
+    * unshelve eapply escapeEq ; tea.
+      apply LRTyEqRefl_.
+    * eapply escapeEqTerm ; tea.
+      now apply LREqTermRefl_.
+    * eapply escapeEqTerm ; tea.
+      now apply LREqTermRefl_.
+  + constructor. 1: escape ; tea.
+    * apply LRTyEqRefl_.
+    * irrelevance.
+    * change [ normList RLA | Γ ||- tl : tList A].
+      irrelevance.
 Qed.
 
-Lemma liftSubst_singleSubst_eq {t u v: term} : t[u]⇑[v..] = t[u[v..]..].
-Proof. now bsimpl. Qed.
-
-Definition natElim {Γ A} (P hz hs : term) {n} {NA : [Γ ||-Nat A]} (p : NatProp NA n) : term.
+Lemma consEqRed {Γ A A' hd hd' tl tl' l}
+  (RA: [Γ ||-< l > A])
+  (RA': [Γ ||-< l > A'])
+  (RLA: [Γ ||-< l > tList A])
+  (RLA': [Γ ||-< l > tList A']) :
+  [RA | Γ ||- A ≅ A'] ->
+  [RLA | Γ ||- tList A ≅ tList A'] ->
+  [RA | Γ ||- hd : A] ->
+  [RA' | Γ ||- hd' : A'] ->
+  [RA | Γ ||- hd ≅ hd' : A] ->
+  [RLA | Γ ||- tl ≅ tl' : tList A] ->
+  [RLA | Γ ||- tl : tList A] ->
+  [RLA' | Γ ||- tl' : tList A'] ->
+  [RLA | Γ ||- tCons A hd tl ≅ tCons A' hd' tl' : tList A ].
 Proof.
-  destruct p.
-  - exact hz.
-  - exact (tApp (tApp hs n) (tNatElim P hz hs n)).
-  - exact (tNatElim P hz hs ne).
+  intros.
+  enough [ normList RLA | Γ ||- tCons A hd tl ≅ tCons A' hd' tl' : _] by irrelevance.
+  econstructor.
+  (* + eapply redtmwf_refl. escape. now apply ty_cons. *)
+  (* + eapply redtmwf_refl. escape. *)
+  (*   eapply ty_conv. 2: symmetry ; eassumption. *)
+  (*   now apply ty_cons. *)
+  (* + eapply convtm_cons; escape; eassumption. *)
+  (* + constructor ; escape ; tea. *)
+  (*   - apply LRTyEqRefl_. *)
+  (*   - irrelevance. *)
+  (*   - irrelevance. *)
+  (*   - change [ normList RLA | Γ ||- tl ≅ tl' : tList A]. *)
+  (*     irrelevance. *)
+Admitted.
+
+Lemma consValid {Γ A hd tl l}
+  {VΓ : [||-v Γ]}
+  {VA : [Γ ||-v<l> A | VΓ]}
+  {VLA : [Γ ||-v<l> tList A | VΓ]}
+  (Vhd : [Γ ||-v<l> hd : A | VΓ | VA ])
+  (Vtl : [Γ ||-v<l> tl : tList A | VΓ | VLA ]) :
+  [Γ ||-v<l> tCons A hd tl : tList A | VΓ | VLA].
+Proof.
+  split; intros.
+  - instValid Vσ.
+    now eapply consRed.
+  - instAllValid Vσ Vσ' Vσσ'.
+    now eapply consEqRed.
+Qed.
+
+Definition mapProp {Γ L l} (A B f x: term) {LL : [Γ ||-List<l> L]} (p : ListProp _ _ LL x) : term.
+Proof.
+  destruct p as [  | | x ].
+  - exact (tNil B).
+  - exact (tCons B (tApp f hd) (tMap A B f tl)).
+  - exact (tMap A B f x).
 Defined.
 
-Section NatElimRed.
-  Context {Γ l P hs hz}
-    (wfΓ : [|- Γ])
-    (NN : [Γ ||-Nat tNat])
-    (RN := LRNat_ _ NN)
-    (RP : [Γ,, tNat ||-<l> P])
-    (RPpt : forall n, [Γ ||-<l> n : _ | RN] -> [Γ ||-<l> P[n..]])
-    (RPext : forall n n' (Rn : [Γ ||-<l> n : _ | RN]),
-      [Γ ||-<l> n' : _ | RN] ->
-      [Γ ||-<l> n ≅ n' : _ | RN] ->
-      [Γ ||-<l> P[n..] ≅ P[n'..] | RPpt _ Rn])
-    (RPz := RPpt _ (zeroRed wfΓ))
-    (Rhz : [Γ ||-<l> hz : P[tZero..] | RPz]) 
-    (RPs : [Γ ||-<l> elimSuccHypTy P])
-    (Rhs : [Γ ||-<l> hs : _ | RPs]).
 
-  Definition natRedElimStmt :=
-    (forall n (Rn : [Γ ||-<l> n : _ | RN]), 
-      [Γ ||-<l> tNatElim P hz hs n : _ | RPpt _ Rn ] ×
-      [Γ ||-<l> tNatElim P hz hs n ≅ tNatElim P hz hs (NatRedTm.nf Rn) : _ | RPpt _ Rn]) ×
-    (forall n (Nn : NatProp NN n) (Rn : [Γ ||-<l> n : _ | RN]), 
-      [Γ ||-<l> tNatElim P hz hs n : _ | RPpt _ Rn ] ×
-      [Γ ||-<l> tNatElim P hz hs n ≅ natElim P hz hs Nn : _ | RPpt _ Rn]).
-
-  Lemma natElimRedAux : natRedElimStmt.
-  Proof.
-    escape.
-    apply NatRedInduction.
-    - intros ? nf red ? nfprop ih.
-      assert [Γ ||-<l> nf : _ | RN]. 1:{
-        econstructor; tea.
-        eapply redtmwf_refl; gen_typing.
-      }
-      eapply redwfSubstTerm.
-      + eapply LRTmRedConv. 
-        2: unshelve eapply ih; tea.
-        eapply RPext. 
-        2: eapply LRTmEqSym.
-        1,2: eapply redwfSubstTerm; tea.
-      + eapply red_natElimSubst; tea.
-        intros; eapply escapeEq; now eapply RPext.
-    - intros. 
-      eapply redSubstTermOneStep.
-      1: eapply osredtm_natElimZero; tea.
-      irrelevance.
-    - intros n Rn ih RSucc; change [Γ ||-<l> n : tNat | RN] in Rn.
-      eapply redSubstTermOneStep.
-      1: eapply osredtm_natElimSucc; tea.
-      1: now escape.
-      eapply simple_appTerm.
-      2: eapply ih.
-      irrelevance0.
-      2: unshelve eapply (appTerm RPs Rhs Rn).
-      now bsimpl.
-    - intros ? [] ?.
-      apply reflect.
-      + apply completeness.
-      + eapply tm_ne_natelim; now first [eassumption|eapply reifyType|eapply reifyTerm].
-      + eapply tm_ne_natelim; now first [eassumption|eapply reifyType|eapply reifyTerm].
-      + now eapply ty_natElim.
-      + now eapply ty_natElim.
-      + eapply convneu_natElim; tea.
-        { eapply escapeEq, LRTyEqRefl_. }
-        { eapply escapeEqTerm; now eapply LREqTermRefl_. }
-        { eapply escapeEqTerm; now eapply LREqTermRefl_. }
-    Unshelve.
-    * tea.
-    * eapply ArrRedTy; now eapply RPpt.
-    * rewrite arr_subst_eq. eapply ArrRedTy.
-      2: rewrite liftSubst_singleSubst_eq; cbn.
-      all: now eapply RPpt.
-    * exact l.
-    * assumption.
-  Qed.
-
-  Lemma natElimRed : forall n (Rn : [Γ ||-<l> n : _ | RN]), [Γ ||-<l> tNatElim P hz hs n : _ | RPpt _ Rn ].
-  Proof. intros. apply (fst natElimRedAux). Qed.
-End NatElimRed.
-
-
-Section NatElimRedEq.
-  Context {Γ l P Q hs hs' hz hz'}
-    (wfΓ : [|- Γ])
-    (NN : [Γ ||-Nat tNat])
-    (RN := LRNat_ _ NN)
-    (RP : [Γ,, tNat ||-<l> P])
-    (RQ : [Γ,, tNat ||-<l> Q])
-    (eqPQ : [Γ,, tNat |- P ≅ Q])
-    (RPpt : forall n, [Γ ||-<l> n : _ | RN] -> [Γ ||-<l> P[n..]])
-    (RQpt : forall n, [Γ ||-<l> n : _ | RN] -> [Γ ||-<l> Q[n..]])
-    (RPQext : forall n n' (Rn : [Γ ||-<l> n : _ | RN]),
-      [Γ ||-<l> n' : _ | RN] ->
-      [Γ ||-<l> n ≅ n' : _ | RN] ->
-      [Γ ||-<l> P[n..] ≅ Q[n'..] | RPpt _ Rn])
-    (RPz := RPpt _ (zeroRed wfΓ))
-    (RQz := RQpt _ (zeroRed wfΓ))
-    (Rhz : [Γ ||-<l> hz : P[tZero..] | RPz]) 
-    (RQhz : [Γ ||-<l> hz' : Q[tZero..] | RQz]) 
-    (RPQhz : [Γ ||-<l> hz ≅ hz' : _ | RPz])
-    (RPs : [Γ ||-<l> elimSuccHypTy P])
-    (RQs : [Γ ||-<l> elimSuccHypTy Q])
-    (Rhs : [Γ ||-<l> hs : _ | RPs])
-    (RQhs : [Γ ||-<l> hs' : _ | RQs])
-    (RPQhs : [Γ ||-<l> hs ≅ hs' : _ | RPs ])
-    .
-
-  Lemma RPext : forall n n' (Rn : [Γ ||-<l> n : _ | RN]),
-      [Γ ||-<l> n' : _ | RN] ->
-      [Γ ||-<l> n ≅ n' : _ | RN] ->
-      [Γ ||-<l> P[n..] ≅ P[n'..] | RPpt _ Rn].
-  Proof.
-    intros. eapply transEq; [| eapply LRTyEqSym ]; eapply RPQext; cycle 1; tea.
-    now eapply LREqTermRefl_.
-    Unshelve. 3,4: eauto. tea.
-  Qed.
-
-  Lemma natElimRedAuxLeft : @natRedElimStmt _ _ P hs hz NN RPpt.
-  Proof.
-    eapply natElimRedAux; tea.
-    + eapply RPext.
-  Qed.
-
-  Lemma natElimRedAuxRight : @natRedElimStmt _ _ Q hs' hz' NN RQpt.
-  Proof.
-    eapply natElimRedAux; tea.
-    + intros. eapply transEq; [eapply LRTyEqSym |]; eapply RPQext; cycle 1; tea.
-      now eapply LREqTermRefl_.
-    Unshelve. 2: eauto. all:tea.
-  Qed.
-
-  Lemma natElimRedEqAux :
-    (forall n n' (Rnn' : [Γ ||-<l> n ≅ n' : _ | RN]) (Rn : [Γ ||-<l> n : _ | RN]) (Rn' : [Γ ||-<l> n' : _ | RN]), 
-      [Γ ||-<l> tNatElim P hz hs n ≅ tNatElim Q hz' hs' n' : _ | RPpt _ Rn ]) ×
-    (forall n n' (Rnn' : NatPropEq NN n n') (Rn : [Γ ||-<l> n : _ | RN]) (Rn' : [Γ ||-<l> n' : _ | RN]), 
-      [Γ ||-<l> tNatElim P hz hs n ≅ tNatElim Q hz' hs' n' : _ | RPpt _ Rn ]).
-  Proof.
-    apply NatRedEqInduction.
-    - intros ?? nfL nfR redL redR ? prop ih RL RR; destruct (NatPropEq_whnf prop).
-      assert [Γ ||-<l> nfL : _ | RN] by (eapply redTmFwd; cycle 1; tea).
-      assert [Γ ||-<l> nfR : _ | RN] by (eapply redTmFwd; cycle 1; tea).
-      eapply LREqTermHelper.
-      * eapply (fst natElimRedAuxLeft).
-      * eapply (fst natElimRedAuxRight).
-      * eapply RPQext. 1: tea.
-        now econstructor.
-      * eapply LRTmEqRedConv.
-        + eapply RPext; tea. 
-          eapply LRTmEqSym; eapply redwfSubstTerm; cycle 1; tea.
-        + unshelve erewrite (redtmwf_det _ _ _ _ _ _ _ _ (NatRedTm.red RL) redL); tea.
-          1: dependent inversion RL; subst; cbn; now eapply NatProp_whnf.
-          unshelve erewrite (redtmwf_det _ _ _ _ _ _ _ _ (NatRedTm.red RR) redR); tea.
-          1: dependent inversion RR; subst; cbn; now eapply NatProp_whnf.
-          now eapply ih.
-        Unshelve. tea.
-    - intros. eapply LREqTermHelper.
-      * unshelve eapply (snd natElimRedAuxLeft); constructor.
-      * unshelve eapply (snd natElimRedAuxRight); tea; constructor.
-      * eapply RPQext; [unshelve eapply zeroRed| unshelve eapply zeroRedEq]; tea.
-      * cbn; irrelevance.
-    - intros ??? ih Rn Rn'. pose proof (succRedInv Rn); pose proof (succRedInv Rn').
-      eapply LREqTermHelper.
-      * unshelve eapply (snd natElimRedAuxLeft); now constructor.
-      * unshelve eapply (snd natElimRedAuxRight); tea; now constructor.
-      * eapply RPQext; [unshelve eapply succRed| unshelve eapply succRedEq]; tea.
-      * cbn.
-        eapply simple_appcongTerm.
-        4: now eapply ih.
-        + irrelevance0. 2: eapply appcongTerm; tea.
-          now bsimpl.
-        + eapply (fst natElimRedAuxLeft).
-        + eapply LRTmRedConv. 2: eapply (fst natElimRedAuxRight).
-          eapply LRTyEqSym; now eapply RPQext.
-        Unshelve. 2,4,5: tea.
-        1: eapply ArrRedTy; now eapply RPpt.
-        rewrite arr_subst_eq. eapply ArrRedTy.
-        2: rewrite liftSubst_singleSubst_eq; cbn.
-        all: now eapply RPpt.
-    - intros ?? neueq ??. escape. inversion neueq.
-      assert [Γ |- P[ne..] ≅ Q[ne'..]]. 1:{
-        eapply escapeEq. eapply RPQext; tea.
-        econstructor.
-        1,2: now eapply redtmwf_refl.
-        2: now constructor.
-        gen_typing.
-      }
-      eapply neuTermEq.
-      + eapply tm_ne_natelim; now first [eassumption|eapply reifyType|eapply reifyTerm].
-      + eapply tm_ne_conv; [|now eapply escape|symmetry; eassumption].
-        eapply tm_ne_natelim; now first [eassumption|eapply reifyType|eapply reifyTerm].
-      + eapply ty_natElim; tea.
-      + eapply ty_conv. 
-        1: eapply ty_natElim; tea.
-        now symmetry.
-      + eapply convneu_natElim ; tea.
-      Unshelve. tea.
-  Qed.
-
-  Lemma natElimRedEq :
-    (forall n n' (Rnn' : [Γ ||-<l> n ≅ n' : _ | RN]) (Rn : [Γ ||-<l> n : _ | RN]) (Rn' : [Γ ||-<l> n' : _ | RN]), 
-      [Γ ||-<l> tNatElim P hz hs n ≅ tNatElim Q hz' hs' n' : _ | RPpt _ Rn ]).
-  Proof. apply natElimRedEqAux. Qed.
-End NatElimRedEq.
-
-
-
-Section NatElimValid.
-  Context {Γ l P}
-    (VΓ : [||-v Γ])
-    (VN := natValid (l:=l) VΓ)
-    (VΓN := validSnoc VΓ VN)
-    (VP : [Γ ,, tNat ||-v<l> P | VΓN]).
-  
-  Lemma elimSuccHypTyValid :
-    [Γ ||-v<l> elimSuccHypTy P | VΓ].
-  Proof.
-    unfold elimSuccHypTy.
-    unshelve eapply PiValid.
-    1: exact VN.
-    eapply simpleArrValid; tea.
-    eapply substLiftS; tea.
-    eapply irrelevanceTm.
-    eapply succValid.
-    eapply irrelevanceTm.
-    change tNat with tNat⟨@wk1 Γ tNat⟩ at 2.
-    eapply var0Valid.
-    Unshelve. all: tea.
-  Qed.
-
-  Context {hz hs}
-    (VPz := substS VP (zeroValid VΓ))
-    (Vhz : [Γ ||-v<l> hz : P[tZero..] | VΓ | VPz]) 
-    (Vhs : [Γ ||-v<l> hs : _ | VΓ | elimSuccHypTyValid]).
-
-
-  Lemma natElimValid {n}
-    (Vn : [Γ ||-v<l> n : tNat | VΓ | VN])
-    (VPn := substS VP Vn)
-    : [Γ ||-v<l> tNatElim P hz hs n : _ | VΓ | VPn].
-  Proof.
-    constructor; intros.
-    - instValid Vσ; cbn.
-      irrelevance0.  1: now rewrite singleSubstComm'.
-      epose proof (Vuσ := liftSubstS' VN Vσ).
-      instValid Vuσ; escape.
-      unshelve eapply natElimRed; tea.
-      + intros m Rm.
-        rewrite up_single_subst. 
-        unshelve eapply validTy; cycle 1; tea.
-        unshelve econstructor; [now bsimpl| now cbn].
-      + rewrite elimSuccHypTy_subst. eapply validTy; tea; eapply elimSuccHypTyValid.
-      + intros m m' Rm Rm' Rmm'; cbn.
-        irrelevance0. 1: now rewrite up_single_subst.
-        rewrite up_single_subst.
-        unshelve eapply validTyExt; cycle 1 ; tea.
-        1,2: unshelve econstructor; [now bsimpl| now cbn].
-        unshelve econstructor; [|now cbn].
-        bsimpl; cbn; eapply reflSubst.
-      + irrelevance.
-      + irrelevance. now rewrite elimSuccHypTy_subst. 
-    - instAllValid Vσ Vσ' Vσσ'.
-      irrelevance0.  1: now rewrite singleSubstComm'.
-      pose (Vuσ := liftSubstS' VN Vσ).
-      pose proof (Vuσ' := liftSubstS' VN Vσ').
-      pose proof (Vuσrea :=  liftSubstSrealign' VN Vσσ' Vσ').
-      pose proof (Vuσσ' := liftSubstSEq' VN Vσσ').
-      instValid Vuσ'; instAllValid Vuσ Vuσrea Vuσσ'; escape.
-      unshelve eapply natElimRedEq; tea; fold subst_term.
-      6-11: irrelevance; now rewrite elimSuccHypTy_subst.
-      3,4: rewrite elimSuccHypTy_subst; eapply validTy; tea; eapply elimSuccHypTyValid.
-      + intros m Rm.
-        rewrite up_single_subst. 
-        unshelve eapply validTy; cycle 1; tea.
-        unshelve econstructor; [now bsimpl| now cbn].
-      + intros m Rm.
-        rewrite up_single_subst. 
-        unshelve eapply validTy; cycle 1; tea.
-        unshelve econstructor; [now bsimpl| now cbn].
-      + intros m m' Rm Rm' Rmm'; cbn.
-        irrelevance0. 1: now rewrite up_single_subst.
-        rewrite up_single_subst.
-        unshelve eapply validTyExt; cycle 1 ; tea.
-        1,2: unshelve econstructor; [now bsimpl| now cbn].
-        unshelve econstructor; [|now cbn].
-        now bsimpl.
-  Qed.
-
-  Lemma natElimZeroValid  : 
-    [Γ ||-v<l> tNatElim P hz hs tZero ≅ hz : _ | VΓ | VPz].
-  Proof.
-    constructor; intros.
-    epose proof (Vuσ := liftSubstS' VN Vσ).
-    instValid Vσ; instValid Vuσ; escape.
-    irrelevance0.  1: now rewrite singleSubstComm'.
-    unshelve eapply (snd (natElimRedAux _ _ _ _ _ _ _ _) _ NatRedTm.zeroR); tea; fold subst_term.
-    7: eapply zeroValid.
-    + intros m Rm.
-      rewrite up_single_subst. 
-      unshelve eapply validTy; cycle 1; tea.
-      unshelve econstructor; [now bsimpl| now cbn].
-    + intros m m' Rm Rm' Rmm'; cbn.
-      irrelevance0. 1: now rewrite up_single_subst.
-      rewrite up_single_subst.
-      unshelve eapply validTyExt; cycle 1 ; tea.
-      1,2: unshelve econstructor; [now bsimpl| now cbn].
-      unshelve econstructor; [|now cbn].
-      bsimpl; cbn; eapply reflSubst.
-    + irrelevance.
-    + rewrite elimSuccHypTy_subst. eapply validTy; tea; eapply elimSuccHypTyValid.
-    + irrelevance. now rewrite elimSuccHypTy_subst. 
-    Unshelve. 4: tea.
-  Qed.
-
-  Lemma natElimSuccValid {n}
-    (Vn : [Γ ||-v<l> n : tNat | VΓ | VN]) 
-    (VPSn := substS VP (succValid _ Vn)) : 
-    [Γ ||-v<l> tNatElim P hz hs (tSucc n) ≅ tApp (tApp hs n) (tNatElim P hz hs n) : _ | VΓ | VPSn].
-  Proof.
-    constructor; intros.
-    epose proof (Vuσ := liftSubstS' VN Vσ).
-    instValid Vσ; instValid Vuσ; escape.
-    irrelevance0.  1: now rewrite singleSubstComm'.
-    pose (NSn := NatRedTm.succR RVn).
-    unshelve eapply (snd (natElimRedAux _ _ _ _ _ _ _ _) _ NSn); tea; fold subst_term.
-    + intros m Rm.
-      rewrite up_single_subst. 
-      unshelve eapply validTy; cycle 1; tea.
-      unshelve econstructor; [now bsimpl| now cbn].
-    + intros m m' Rm Rm' Rmm'; cbn.
-      irrelevance0. 1: now rewrite up_single_subst.
-      rewrite up_single_subst.
-      unshelve eapply validTyExt; cycle 1 ; tea.
-      1,2: unshelve econstructor; [now bsimpl| now cbn].
-      unshelve econstructor; [|now cbn].
-      bsimpl; cbn; eapply reflSubst.
-    + irrelevance.
-    + rewrite elimSuccHypTy_subst. eapply validTy; tea; eapply elimSuccHypTyValid.
-    + irrelevance. now rewrite elimSuccHypTy_subst. 
-    + now eapply succRed.
-  Qed.
-
-End NatElimValid.
-
-Lemma natElimCongValid {Γ l P Q hz hz' hs hs' n n'}
-    (VΓ : [||-v Γ])
-    (VN := natValid (l:=l) VΓ)
-    (VΓN := validSnoc VΓ VN)
-    (VP : [Γ ,, tNat ||-v<l> P | VΓN])
-    (VQ : [Γ ,, tNat ||-v<l> Q | VΓN])
-    (VPQ : [Γ ,, tNat ||-v<l> P ≅ Q | VΓN | VP])
-    (VPz := substS VP (zeroValid VΓ))
-    (VQz := substS VQ (zeroValid VΓ))
-    (Vhz : [Γ ||-v<l> hz : P[tZero..] | VΓ | VPz]) 
-    (Vhz' : [Γ ||-v<l> hz' : Q[tZero..] | VΓ | VQz])
-    (Vheqz : [Γ ||-v<l> hz ≅ hz' : P[tZero..] | VΓ | VPz])
-    (VPs := elimSuccHypTyValid VΓ VP)
-    (VQs := elimSuccHypTyValid VΓ VQ)
-    (Vhs : [Γ ||-v<l> hs : _ | VΓ | VPs]) 
-    (Vhs' : [Γ ||-v<l> hs' : _ | VΓ | VQs])
-    (Vheqs : [Γ ||-v<l> hs ≅ hs' : _ | VΓ | VPs]) 
-    (Vn : [Γ ||-v<l> n : _ | VΓ | VN])
-    (Vn' : [Γ ||-v<l> n' : _ | VΓ | VN])
-    (Veqn : [Γ ||-v<l> n ≅ n' : _ | VΓ | VN])
-    (VPn := substS VP Vn) :
-    [Γ ||-v<l> tNatElim P hz hs n ≅ tNatElim Q hz' hs' n' : _ | VΓ | VPn].
+Lemma mapRedAux {Γ A B f l}
+  {RA : [Γ ||-<l> A]}
+  {RB : [Γ ||-<l> B]}
+  {LA : [Γ ||-List<l> tList A]}
+  (LA' := normList0 LA : [Γ ||-List<l> tList A])
+  (RLA :=  LRList' LA' : [Γ ||-<l> tList A] )
+  {RLB : [Γ ||-<l> tList B]}
+  {RFAB : [Γ ||-<l> arr A B]}
+  (Rf: [Γ ||-<l> f : arr A B | RFAB]) :
+  (forall x (Rx: ListRedTm _ _ LA' x),
+        [Γ ||-<l> tMap A B f x : tList B | RLB] ×
+        [Γ ||-<l> tMap A B f x ≅ tMap A B f (ListRedTm.nf Rx) : tList B | RLB])
+    ×
+    (forall x (Rx: ListProp _ _ LA' x),
+        [Γ ||-<l> tMap A B f x : tList B | RLB] ×
+          [Γ ||-<l> tMap A B f x ≅ mapProp A B f x Rx : tList B | RLB]).
 Proof.
-  constructor; intros.
-  pose (Vuσ := liftSubstS' VN Vσ).
-  instValid Vσ; instValid Vuσ; escape.
-  irrelevance0.  1: now rewrite singleSubstComm'.
-  unshelve eapply natElimRedEq; tea; fold subst_term.
-  6-11: irrelevance; now rewrite elimSuccHypTy_subst.
-  3,4: rewrite elimSuccHypTy_subst; eapply validTy; tea; eapply elimSuccHypTyValid.
-  + intros m Rm.
-    rewrite up_single_subst. 
-    unshelve eapply validTy; cycle 1; tea.
-    unshelve econstructor; [now bsimpl| now cbn].
-  + intros m Rm.
-    rewrite up_single_subst. 
-    unshelve eapply validTy; cycle 1; tea.
-    unshelve econstructor; [now bsimpl| now cbn].
-  + intros m m' Rm Rm' Rmm'; cbn.
-    irrelevance0. 1: now rewrite up_single_subst.
-    rewrite up_single_subst.
-    eapply transEq; cycle 1.
-    - unshelve eapply validTyEq. 
-      7: tea. 1: tea.
-      unshelve econstructor; [now bsimpl| now cbn].
-    - unshelve eapply validTyExt; cycle 1 ; tea.
-    1,2: unshelve econstructor; [now bsimpl| now cbn].
-    unshelve econstructor; [|now cbn].
-    bsimpl. eapply reflSubst.
-    Unshelve. 1: tea.
-    eapply validTy; tea.
-    unshelve econstructor; [| now cbn]; now bsimpl.
+  escape.
+  apply ListRedInduction.
+  - intros.
+    apply redSubstTerm. 1: intuition.
+    apply redtm_map ; tea.
+    eapply redtm_conv. 1: now apply red.
+    destruct LA. cbn in *. gen_typing.
+  - intros.
+    apply redSubstTerm. 1: now apply nilRed.
+    eapply redtm_map_nil ; tea.
+    unshelve eapply escapeEq.
+    3: eassumption.
+  - admit.
+  - admit.
+Admitted.
+
+Lemma mapEqRedAux {Γ A A' B B' f f' l}
+  {RA : [Γ ||-<l> A]}
+  {RA' : [Γ ||-<l> A']}
+  {REA : [RA | Γ ||- A ≅ A' ]}
+  {RB : [Γ ||-<l> B]}
+  {RB' : [Γ ||-<l> B']}
+  {REB : [RB | Γ ||- B ≅ B' ]}
+  {LA : [Γ ||-List<l> tList A]}
+  (LA_ := normList0 LA : [Γ ||-List<l> tList A])
+  {LA' : [Γ ||-List<l> tList A']}
+  (LA'_ := normList0 LA' : [Γ ||-List<l> tList A'])
+  (RLA := LRList' LA_ : [Γ ||-<l> tList A] )
+  {RLB : [Γ ||-<l> tList B]}
+  {RLB' : [Γ ||-<l> tList B']}
+  {RELA : [Γ ||-<l> tList A ≅ tList A' | RLA ]}
+  {RELB : [Γ ||-<l> tList B ≅ tList B' | RLB ]}
+  {RFAB : [Γ ||-<l> arr A B]}
+  {RFAB' : [Γ ||-<l> arr A' B']}
+  (Rf: [Γ ||-<l> f : arr A B | RFAB])
+  (Rf': [Γ ||-<l> f' : arr A' B' | RFAB']) :
+  (forall x x' (Rxx': ListRedTmEq _ _ LA_ x x'),
+        [Γ ||-<l> tMap A B f x ≅ tMap A' B' f' x' : tList B | RLB])
+    ×
+    (forall x x' (Rxx': ListPropEq _ _ LA_ x x'),
+          [Γ ||-<l> tMap A B f x ≅ tMap A' B' f' x' : tList B | RLB]).
+  apply ListRedEqInduction.
+  - intros.
+    eapply LREqTermHelper.
+    4: eassumption.
+    1: now unshelve eapply mapRedAux.
+    2: eassumption.
+    unshelve epose (Ru' := _ : ListRedTm Γ (tList A') LA'_ u).
+    {
+      change ([LRList' LA'_ | Γ ||- u : _ ]).
+      unshelve eapply (fst (ListIrrelevanceTm LA_ LA'_ _ _ _) _ Ru).
+      1-2: now escape.
+      eapply LRIrrelevantCum.
+      3: {
+        cbn. now irrelevanceRefl.
+      }
+      1-2: eapply LRAd.adequate.
+    }
+    replace (ListRedTm.nf Ru) with (ListRedTm.nf Ru').
+    2: destruct Ru; reflexivity.
+    now unshelve eapply mapRedAux.
+    Unshelve. now tea.
+  - intros.
+    eapply LREqTermHelper.
+    3: eassumption.
+    + unshelve eapply mapRedAux ; tea.
+      econstructor ; tea.
+      irrelevance.
+    + unshelve eapply mapRedAux ; tea.
+      econstructor ; tea.
+      eapply transEq ; tea.
+      unshelve eapply LRTyEqSym. 3: eassumption.
+    + cbn. now eapply nilEqRed.
+  - intros.
+    eapply LREqTermHelper.
+    3: eassumption.
+    all: admit.
+  - admit. (* see Neutral.v *)
+Admitted.
+
+(* TODO: move; also wk_arr vs arr_wk *)
+Lemma subst_arr A B σ : (arr A B)[σ] = arr (subst_term σ A) (subst_term σ B).
+Proof. now bsimpl. Qed.
+
+Lemma mapValid {Γ A B f x l}
+  {VΓ : [||-v Γ]}
+  {VA : [Γ ||-v<l> A | VΓ]}
+  {VB : [Γ ||-v<l> B | VΓ]}
+  {VLA : [Γ ||-v<l> tList A | VΓ]}
+  {VLB : [Γ ||-v<l> tList B | VΓ]}
+  {VFAB : [Γ ||-v<l> arr A B | VΓ]}
+  (Vf : [Γ ||-v<l> f : arr A B | VΓ | VFAB ])
+  (Vx : [Γ ||-v<l> x : tList A | VΓ | VLA ]) :
+  [Γ ||-v<l> tMap A B f x : tList B | VΓ | VLB].
+Proof.
+  split; intros.
+  - instValid Vσ.
+    unshelve eapply (fst (mapRedAux _)) ; tea ; fold subst_term.
+    + now eapply invLRList.
+    + now eapply ArrRedTy.
+    + irrelevance0 ; tea.
+      apply subst_arr.
+    + change [normList RVLA | Δ ||- x[σ] : (tList A)[σ]]. irrelevance.
+
+  - instAllValid Vσ Vσ' Vσσ'.
+    unshelve eapply (fst (mapEqRedAux _ _)) ; tea ; fold subst_term.
+    + now eapply invLRList.
+    + now eapply invLRList.
+    + irrelevance.
+    + now eapply ArrRedTy.
+    + now eapply ArrRedTy.
+    + irrelevance0 ; tea.
+      apply subst_arr.
+    + irrelevance0 ; tea.
+      apply subst_arr.
+    + change [normList RVLA | Δ ||- x[σ] ≅ x[σ'] : _]. irrelevance.
 Qed.
 
-Lemma elimSuccHypTyCongValid {Γ l P P'}
-    (VΓ : [||-v Γ])
-    (VN := natValid (l:=l) VΓ)
-    (VΓN := validSnoc VΓ VN)
-    (VP : [Γ ,, tNat ||-v<l> P | VΓN])
-    (VP' : [Γ ,, tNat ||-v<l> P' | VΓN])
-    (VeqP : [Γ ,, tNat ||-v<l> P ≅ P' | VΓN | VP]) :
-    [Γ ||-v<l> elimSuccHypTy P ≅ elimSuccHypTy P' | VΓ | elimSuccHypTyValid VΓ VP].
-  Proof.
-    unfold elimSuccHypTy.
-    eapply irrelevanceEq.
-    assert [Γ,, tNat ||-v< l > P'[tSucc (tRel 0)]⇑ | validSnoc VΓ VN]. 1:{
-      eapply substLiftS; tea.
-      eapply irrelevanceTm.
-      eapply succValid.
-      eapply irrelevanceTm.
-      change tNat with tNat⟨@wk1 Γ tNat⟩ at 2.
-      eapply var0Valid.
-    }
-    eapply PiCong.
-    - eapply simpleArrValid; tea.
-    - eapply reflValidTy.
-    - eapply simpleArrCongValid; tea.
-      eapply substLiftSEq; tea.
-    Unshelve. all: tea.
-    unshelve eapply irrelevanceTm; tea.
-    2: eapply succValid.
-    unshelve eapply irrelevanceTm'.
-    5: unshelve eapply var0Valid; tea.
-    now bsimpl.
-  Qed.
+(* TODO: also missing cong valid! *)
+(* TODO: and then the equations (tMap A A' f l ≅ l when f ≅ id  *)
 
-End Nat.
+(* mutual induction on listRed/listProp *)
+
+
+
+
+
+End List.
